commit

Projects/Util/Serializable/Serializer.lean
@@ -186,6 +186,35 @@ theorem mul_two_lor_one_eq {n : ℕ} : n * 2 ||| 1 = n * 2 + 1 := by
 theorem mul_two_add_one_lor_one_eq {n : ℕ} : (n * 2 + 1) ||| 1 = n * 2 + 1 := by
   rw [lor_one_eq_ite]; simp
 
+theorem mod_self_pow_succ {n m : ℕ} (hn : n ≠ 1) (hm : m ≠ 0) : n % n ^ (m + 1) = n := by
+  cases n; simp; nm n; simp at hn; apply Nat.mod_eq_of_lt
+  apply lt_self_pow₀ <;> simp <;> omega
+
+theorem beq_eq_eq {n m : ℕ} : (n == m) = decide (n = m) := rfl
+
+theorem mod_two_eq_one_iff_odd {n : ℕ} : n % 2 = 1 ↔ Odd n := by
+  rw [Nat.odd_iff]
+
+theorem mod_two_eq_zero_iff_even {n : ℕ} : n % 2 = 0 ↔ Even n := by
+  rw [Nat.even_iff]
+
+theorem testBit_eq_odd {n i : ℕ} : n.testBit i = decide (Odd (n >>> i)) := by
+  simp [-decide_shiftRight_mod_two_eq_one, testBit, beq_eq_eq, mod_two_eq_one_iff_odd]
+
+theorem ne_zero_of_odd {n : ℕ} (h : Odd n) : n ≠ 0 := by
+  rintro rfl; simp at h
+
+theorem pos_of_odd {n : ℕ} (h : Odd n) : 0 < n :=
+  pos_of_ne_zero # ne_zero_of_odd h
+
+@[simp]
+theorem sum_min_left {n m : ℕ} : n - min n m = n - m := by
+  omega
+
+@[simp]
+theorem sum_min_right {n m : ℕ} : n - min m n = n - m := by
+  omega
+
 -- #check 0 #exit
 
 end Nat
@@ -198,8 +227,43 @@ variable {xs ys zs : List α}
 theorem range_add' {n m : Nat} : range (n + m) = range m ++ (range n).map (m + ·) := by
   rw [add_comm, range_add]
 
-theorem range_succ' {n : ℕ} : List.range (n + 1) = 0 :: (List.range n).map (· + 1) := by
+theorem range_succ' {n : ℕ} : range (n + 1) = 0 :: (range n).map (· + 1) := by
   rw [range_add']; simp; omega
+
+attribute [-simp] List.getElem!_eq_getElem?_getD
+
+@[simp]
+theorem map_getElem!_range_length [ha : Inhabited α] :
+(range xs.length).map (xs[·]!) = xs := by
+  apply ext_getElem <;> simp
+
+theorem map_getElem!_range_of_le_length [ha : Inhabited α] {n : ℕ}
+(h : n ≤ xs.length) : (range n).map (xs[·]!) = xs.take n := by
+  apply ext_getElem <;> simp; omega
+
+theorem map_getElem!_range_of_length_le [ha : Inhabited α] {n : ℕ}
+(h : xs.length ≤ n) : (range n).map (xs[·]!) = xs ++ replicate (n - xs.length) default := by
+  obtain ⟨n, rfl⟩ := Nat.exists_eq_add_of_le h; simp [range_add]
+
+theorem map_getElem!_range [ha : Inhabited α] {n : ℕ} :
+(range n).map (xs[·]!) = xs.take n ++ replicate (n - xs.length) default := by
+  by_cases h : n ≤ xs.length
+  · simp [Nat.sub_eq_zero_of_le h, map_getElem!_range_of_le_length h]
+  · rw [map_getElem!_range_of_length_le # by omega]; simp; omega
+
+theorem foldr_apply {f : α → β → β} {z : β}
+(g₁ : β → γ) (g₂ : γ → β) (h : ∀ ⦃x⦄, g₂ (g₁ x) = x) :
+xs.foldr f z = g₂ (xs.foldr (λ x acc => g₁ # f x # g₂ acc) (g₁ z)) := by
+  induction xs <;> grind
+
+theorem foldl_apply {f : β → α → β} {z : β}
+(g₁ : β → γ) (g₂ : γ → β) (h : ∀ ⦃x⦄, g₂ (g₁ x) = x) :
+xs.foldl f z = g₂ (xs.foldl (λ acc x => g₁ # f (g₂ acc) x) (g₁ z)) := by
+  simp_rw [foldl_eq_foldr_reverse, foldr_apply _ _ h]
+
+@[simp]
+theorem take_take_same {n : ℕ} : (xs.take n).take n = xs.take n := by
+  rw [take_take]; simp
 
 -- #check 0 #exit
 
@@ -210,6 +274,35 @@ namespace Bit
 @[simp]
 theorem ofBool_eq_iff {b₁ b₂} : ofBool b₁ = ofBool b₂ ↔ b₁ = b₂ := by
   cases b₁ <;> cases b₂ <;> simp
+
+@[simp] theorem ofBool_false : ofBool false = 0 := rfl
+@[simp] theorem ofBool_true : ofBool true = 1 := rfl
+@[simp] theorem toBool_0 : toBool 0 = false := rfl
+@[simp] theorem toBool_1 : toBool 1 = true := rfl
+
+@[simp]
+theorem ofBool_eq_zero_iff {b : Bool} : ofBool b = 0 ↔ b = false := by
+  cases b <;> simp
+
+@[simp]
+theorem ofBool_eq_one_iff {b : Bool} : ofBool b = 1 ↔ b = true := by
+  cases b <;> simp
+
+@[simp]
+theorem toBool_eq_false_iff {b : Bit} : b.toBool = false ↔ b = 0 := by
+  cases b <;> simp
+
+@[simp]
+theorem toBool_eq_true_iff {b : Bit} : b.toBool = true ↔ b = 1 := by
+  cases b <;> simp
+
+@[simp]
+theorem toBool_ofBool {b : Bool} : (ofBool b).toBool = b := by
+  cases b <;> rfl
+
+@[simp]
+theorem ofBool_toBool {b : Bit} : ofBool b.toBool = b := by
+  cases b <;> rfl
 
 -- #check 0 #exit
 
@@ -276,10 +369,6 @@ theorem shiftLeft_one_eq_mul_two : x <<< 1 = x * 2 := by
   rw [shiftLeft_eq_mul_twoPow]; congr; simp [twoPow]; clear! w x
   rw [←BitVec.toFin_inj]; simp; ext; simp; rw [Nat.shiftLeft_eq]; simp
 
-theorem mod_self_pow_succ {n m : ℕ} (hn : n ≠ 1) (hm : m ≠ 0) : n % n ^ (m + 1) = n := by
-  cases n; simp; nm n; simp at hn; apply Nat.mod_eq_of_lt
-  apply lt_self_pow₀ <;> simp <;> omega
-
 theorem mul_two_or_one_eq : x * 2 ||| 1 = x * 2 + 1 := by
   rcases x with ⟨⟨x, h⟩⟩
   rw [←BitVec.toFin_inj]
@@ -310,7 +399,7 @@ theorem mul_two_or_one_eq : x * 2 ||| 1 = x * 2 + 1 := by
   rw [Nat.mod_eq_of_lt]
   omega
 
-theorem foldr_eq_add_toBits {bs : List Bit} {z : BitVec w} :
+theorem foldr_eq_add_ofBits {bs : List Bit} {z : BitVec w} :
 bs.foldr (λ bit (x : BitVec w) => (x <<< 1) ||| ofBit w bit) z =
 (z <<< bs.length) + ofBits w bs := by
   unfold ofBits
@@ -326,311 +415,423 @@ bs.foldr (λ bit (x : BitVec w) => (x <<< 1) ||| ofBit w bit) z =
   simp_rw [mul_two_or_one_eq]
   grind
 
+theorem ofBits_snoc_eq_add_ofBits {bs : List Bit} {b : Bit} :
+ofBits w (bs ++ [b]) = ofBit _ b <<< bs.length + ofBits _ bs := by
+  rw [ofBits]; simp [foldr_eq_add_ofBits]
+
+attribute [-simp] List.getElem!_eq_getElem?_getD
+
 @[simp]
-theorem ofBits_snoc {bs : List Bit} {b : Bit} :
-ofBits (w + 1) (bs ++ [b]) = ofBit _ b <<< bs.length + ofBits _ bs := by
-  rw [ofBits]; simp [foldr_eq_add_toBits]
+theorem getElem_zero_ofBit {b h} : (ofBit w b)[0]'h = b.toBool := by
+  cases b <;> simp [ofBit]
+
+@[simp]
+theorem getElem_succ_ofBit {i : ℕ} {b h} : (ofBit w b)[i + 1]'h = false := by
+  cases b <;> simp [ofBit]
+
+@[simp]
+theorem getElem_ofBits {bs} {i : ℕ} {h} : (ofBits w bs)[i]'h = bs[i]! := by
+  rw [ofBits]
+  generalize hz : (0 : BitVec w) = z; symm at hz
+  trans (z <<< bs.length)[i] || bs[i]!.toBool
+  on_goal 2 => simp [hz]
+  clear hz
+  rw [Bool.eq_iff_iff]
+  simp
+  induction bs generalizing i z <;> simp
+  nm b bs ih
+  cases i <;> simp
+  nm i
+  rw [ih]; clear ih
+  grind
+
+theorem foldr_eq_or_ofBits {bs : List Bit} {z : BitVec w} :
+bs.foldr (λ bit (x : BitVec w) => (x <<< 1) ||| ofBit w bit) z =
+(z <<< bs.length) ||| ofBits w bs := by
+  rw [foldr_eq_add_ofBits]
+  apply add_eq_or_of_and_eq_zero
+  ext i h
+  simp
+  intro h₁
+  obtain ⟨i, rfl⟩ := Nat.exists_eq_add_of_le h₁
+  simp
+
+theorem ofBits_snoc_eq_or_ofBits {bs : List Bit} {b : Bit} :
+ofBits w (bs ++ [b]) = ofBit _ b <<< bs.length ||| ofBits _ bs := by
+  rw [ofBits]; simp [foldr_eq_or_ofBits]
 
 @[simp]
 theorem length_toBits : x.toBits.length = w := by
   simp [toBits]
 
+theorem odd_shiftRight_toNat_iff {i : ℕ} : Odd (x.toNat >>> i) ↔ ∃ (h : i < w), x[i] := by
+  rcases x with ⟨⟨x, h⟩⟩
+  simp [Nat.shiftRight_eq_div_pow, Nat.testBit_eq_odd]
+  intro h₁
+  replace h₁ := Nat.pos_of_odd h₁
+  simp [Nat.div_pos_iff] at h₁
+  replace h₁ := lt_of_le_of_lt h₁ h
+  rwa [Nat.pow_lt_pow_iff_right (by simp)] at h₁
+
+theorem lowestBit_shiftRight {i : ℕ} :
+(x >>> i).lowestBit = if h : i < w then .ofBool x[i] else 0 := by
+  simp [lowestBit, odd_shiftRight_toNat_iff]; split_ifs with h <;> simp [h]
+
+theorem toBits_eq_map_getElem : x.toBits = (List.range w).attach.map
+λ ⟨i, h⟩ => .ofBool # x[i]'(by grind) := by
+  simp [toBits]
+  rw [List.map_eq_map_attach]
+  congr
+  ext y
+  rcases y with ⟨i, h⟩
+  simp at h
+  simp [lowestBit_shiftRight, h]
+
+@[simp]
+theorem getElem_cons_last {b h} : (cons b x)[w] = b := by
+  simp [getElem_cons]
+
+@[simp]
+theorem ofBits_toBits : ofBits _ x.toBits = x := by
+  induction x
+  · simp
+  clear! w x
+  nm w b x ih
+  simp
+  ext i h
+  rw [ofBits_snoc_eq_or_ofBits]
+  rw [Bool.eq_iff_iff]
+  simp
+  by_cases h₁ : i = w
+  · subst h₁
+    simp
+  replace h₁ : i < w; omega
+  simp [show ¬(w ≤ i) by omega]
+  rw [getElem_cons, dif_neg (by omega)]
+  rw [toBits_eq_map_getElem]
+  simp
+  rw [List.getElem!_eq_getElem (by simpa)]
+  simp
+
+@[simp]
+theorem toBits_eq_iff : x.toBits = y.toBits ↔ x = y := by
+  symm; constructor; tauto; intro h
+  replace h := congrArg (ofBits w) h
+  simp at h; exact h
+
+@[simp]
+theorem list_subset_zero_one {bs : List Bit} : bs ⊆ [0, 1] := by
+  intro; simp
+
+@[simp]
+theorem w_zero_eq {x : BitVec 0} : x = (BitVec.ofNat 0 0) := by
+  ext; omega
+
+theorem toBits_ofBits {bs : List Bit} : (ofBits w bs).toBits =
+bs.take w ++ .replicate (w - bs.length) 0 := by
+  simp [toBits_eq_map_getElem, List.map_getElem!_range]
+
+theorem toBits_ofBits_of_length_eq {bs : List Bit} (h : bs.length = w) :
+(ofBits w bs).toBits = bs := by
+  simp [toBits_ofBits, h]
+
+theorem toBits_ofBits_of_length_le {bs : List Bit} (h : bs.length ≤ w) :
+(ofBits w bs).toBits = bs ++ .replicate (w - bs.length) 0 := by
+  simp [toBits_ofBits, h]
+
+theorem toBits_ofBits_of_le_length {bs : List Bit} (h : w ≤ bs.length) :
+(ofBits w bs).toBits = bs.take w := by
+  simp [toBits_ofBits, h]
+
+@[simp]
+theorem toBits_eq_nil_iff : x.toBits = [] ↔ w = 0 := by
+  rw [List.eq_nil_iff_length_eq_zero, length_toBits]
+
 -- #check 0 #exit
 
--- @[simp]
--- theorem ofBits_toBits : ofBits _ x.toBits = x := by
---   induction x
---   ·
---     simp
---   clear! w x
---   nm w b x ih
---   simp
--- 
+end BitVec
+
+namespace UInt8
+
+def ofBit (b : Bit) : UInt8 :=
+  match b with
+  | 0 => 0
+  | 1 => 1
+
+def lowestBit (x : UInt8) : Bit :=
+  .ofBool # Odd x.toNat
+
+def ofBits (bs : List Bit) : UInt8 :=
+  bs.foldr (λ bit x => (x <<< 1) ||| ofBit bit) 0
+
+def toBits (x : UInt8) : List Bit :=
+  List.range 8 |>.map # λ n => (x >>> ofNat n).lowestBit
+
+-----
+
+variable {x y z : UInt8}
+variable {bs : List Bit}
+
+attribute [simp] UInt8.toNat_lt_size
+
+@[simp]
+theorem mk_eq_mk_iff {x y : BitVec 8} : (⟨x⟩ : UInt8) = ⟨y⟩ ↔ x = y := by
+  constructor
+  · rintro ⟨⟩; rfl
+  · rintro rfl; rfl
+
+theorem eq_iff_mk : x = y ↔ x.toBitVec = y.toBitVec := by
+  cases x; cases y; simp
+
+@[simp]
+theorem ofNatLT_eq_ofNatLT_iff {n m hn hm} : ofNatLT n hn = ofNatLT m hm ↔ n = m := by
+  simp_rw [ofNatLT, mk_eq_mk_iff]; simp
+
+attribute [-simp] List.getElem!_eq_getElem?_getD
+attribute [-simp] Bit.ofBool
+
+@[simp]
+theorem ofBit_eq_mk {b} : ofBit b = ⟨.ofBit _ b⟩ := by
+  cases b <;> rfl
+
+@[simp]
+theorem lowestBit_mk {x : BitVec 8} : lowestBit ⟨x⟩ = x.lowestBit := rfl
+
+theorem or_eq_mk : x ||| y = ⟨x.toBitVec ||| y.toBitVec⟩ := rfl
+
+@[simp]
+theorem ofBits_eq_mk {bs : List Bit} : ofBits bs = ⟨.ofBits _ bs⟩ := by
+  simp [eq_iff_mk, ofBits, BitVec.ofBits]
+  rw [List.foldr_apply toBitVec ofBitVec]; simp
+  rintro ⟨x⟩; simp
+
+@[simp]
+theorem toBitVec_eq_iff : x.toBitVec = y.toBitVec ↔ x = y := by
+  cases x; cases y; simp
+
+@[simp]
+theorem toBits_eq_mk : x.toBits = x.toBitVec.toBits := rfl
+
+end UInt8
+
+namespace ByteArray
+
+def ofBits' (acc : List UInt8) (bs : List Bit) : List UInt8 :=
+  if bs = [] then acc else
+  match _h : bs.splitAt 8 with
+  | (xs, bs') => ofBits' (.ofBits xs :: acc) bs'
+termination_by bs.length
+decreasing_by have : bs.length ≠ 0; simpa; grind
+
+def ofBits (bs : List Bit) : ByteArray :=
+  ⟨⟨ofBits' [] bs |>.reverse⟩⟩
+
+def toBits (bs : ByteArray) : List Bit :=
+  bs.1.1.flatMap UInt8.toBits
+
+-----
+
+theorem empty_def : (∅ : ByteArray) = ⟨⟨[]⟩⟩ := rfl
+
+@[simp]
+theorem ofBits_nil : ofBits [] = ∅ := by
+  ext <;> simp [ofBits, ofBits']
+
+@[simp]
+theorem ofBits'_nil {acc} : ofBits' acc [] = acc := by
+  simp [ofBits']
+
+@[simp]
+theorem ofBits_toBits {bs : ByteArray} : ofBits bs.toBits = bs := by
+  rcases bs with ⟨⟨bs⟩⟩
+  simp [ofBits, toBits]
+  suffices h : ∀ acc, ofBits' acc (bs.flatMap UInt8.toBits) = bs.reverse ++ acc
+  · specialize h []
+    simp at h
+    simp [h]
+  intro acc
+  induction bs generalizing acc
+  · simp
+  nm x bs ih
+  simp
+  unfold ofBits'
+  simp [ih]
+
+@[simp] theorem toBits_empty : empty.toBits = [] := rfl
+
+theorem ofBits'_of_length_le_8 {bs₁ : List UInt8} {bs₂ : List Bit}
+(h₁ : bs₂ ≠ []) (h₂ : bs₂.length ≤ 8) : ofBits' bs₁ bs₂ = .ofBits bs₂ :: bs₁ := by
+  unfold ofBits'; simp [h₁]; rw [List.take_eq_self_of_le h₂, List.drop_eq_nil_of_le h₂]; simp
+
+theorem ofBits'_eq_append {bs₁ bs₂} : ofBits' bs₁ bs₂ = ofBits' [] bs₂ ++ bs₁ := by
+  generalize hn : bs₂.length = n
+  induction n using Nat.strong_induction_on generalizing bs₁ bs₂
+  nm n ih
+  cases n
+  · simp at hn
+    simp [hn]
+  nm n
+  have h₁ : bs₂ ≠ []; grind
+  nth_rw 2 [ofBits']
+  rw [ofBits']
+  simp [h₁]
+  nth_rw 2 [@ih (bs₂.drop 8).length (by grind) _ (bs₂.drop 8) rfl]
+  rw [@ih (bs₂.drop 8).length (by grind) _ (bs₂.drop 8) rfl]
+  simp
+
+@[simp]
+theorem toBits_ofBits {bs : List Bit} :
+(ofBits bs).toBits = bs ++ .replicate ((8 - bs.length % 8) % 8) 0 := by
+  generalize hn : bs.length = n
+  induction n using Nat.strong_induction_on generalizing bs
+  nm n ih; subst hn
+  by_cases h₁ : bs = []
+  · simp [h₁]
+  by_cases h₂ : bs.length = 8
+  · simp [h₂]
+    simp [ofBits, toBits, ofBits'_of_length_le_8 h₁ # by omega]
+    rw [BitVec.toBits_ofBits_of_length_eq h₂]
+  by_cases h₃ : bs.length < 8
+  · clear ih
+    rw [Nat.mod_eq_of_lt h₃]
+    simp [ofBits, toBits, ofBits'_of_length_le_8 h₁ # le_of_lt h₃]
+    rw [BitVec.toBits_ofBits_of_length_le # by omega]
+    simp
+    rw [Nat.mod_eq_of_lt]
+    have h₄ : bs.length ≠ 0; grind
+    omega
+  replace h₂ : 8 < bs.length; omega
+  clear h₃
+  simp [ofBits, toBits]
+  unfold ofBits'
+  simp [h₁]
+  generalize h₃ : bs.drop 8 = bs'
+  have h₄ : bs'.length < bs.length
+  · subst h₃; simp; grind
+  specialize @ih _ h₄ bs' rfl
+  have h₅ : bs'.length % 8 = bs.length % 8
+  · subst h₃
+    simp
+    omega
+  rw [h₅] at ih
+  have h₆ := bs.take_append_drop 8
+  rw [h₃] at h₆
+  nth_rw 2 [←h₆]
+  rw [List.append_assoc]
+  rw [←ih]; clear ih
+  rw [ofBits'_eq_append]
+  simp
+  congr 1
+  rw [BitVec.toBits_ofBits]
+  simp; omega
+
 -- #check 0 #exit
--- 
--- @[simp]
--- theorem toBits_eq_iff : x.toBits = y.toBits ↔ x = y := by
---   sorry
--- 
--- -- #check 0 #exit
--- 
--- @[simp]
--- theorem length_toBits : x.toBits.length = 8 := by
---   simp [toBits]
--- 
--- @[simp]
--- theorem list_subset_zero_one {bs : List Bit} : bs ⊆ [0, 1] := by
---   intro; simp
--- 
--- theorem toBits_ofBits_of_length_eq_8 (h : bs.length = 8) : (ofBits bs).toBits = bs := by
---   sorry
--- 
--- theorem toBits_ofBits_of_length_le_8 (h : bs.length ≤ 8) :
--- (ofBits bs).toBits = bs ++ List.replicate (8 - bs.length) 0 := by
---   sorry
--- 
--- @[simp]
--- theorem toBits_ne_nil : x.toBits ≠ [] := by
---   apply ne_of_congr (·.length); simp
--- 
--- @[simp]
--- theorem toBits_ofBits {bs : List Bit} :
--- (ofBits bs).toBits = bs ++ .replicate (8 - bs.length) 0 := by
---   simp [ofBits, toBits]
---   sorry
--- 
+
+end ByteArray
+
+structure Serializer where
+  bytes : ByteArray
+  curByte : UInt8
+  bitMask : UInt8
+deriving DecidableEq
+
+namespace Serializer
+
+abbrev Ser := StateM Serializer
+
+def empty : Serializer where
+  bytes := ∅
+  curByte := 0
+  bitMask := 1
+
+instance : EmptyCollection Serializer := ⟨empty⟩
+theorem empty_def : (∅ : Serializer) = empty := rfl
+
+def flush' : Ser Unit := modify # λ s =>
+  { bytes := s.bytes.push s.curByte
+    curByte := 0
+    bitMask := 1
+  }
+
+def flush : Ser Unit := do
+  bif (←get).bitMask != 0 then pure () else flush'
+
+def writeBit' (b : Bit) : Ser Unit := modify # λ s =>
+  { bytes := s.bytes
+    curByte := match b with
+      | .B₀ => s.curByte
+      | .B₁ => s.curByte ||| s.bitMask
+    bitMask := s.bitMask <<< 1
+  }
+
+def writeBit (b : Bit) : Ser Unit := do
+  writeBit' b; flush
+
+def writeBits (bs : List Bit) : Ser Unit :=
+  bs.forM writeBit
+
+def getOutput : Ser ByteArray := do
+  flush; gets (·.bytes)
+
+def ofBits (bs : List Bit) : Serializer :=
+  StateT.run (m := Id) (writeBits bs) ∅ |>.2
+
 -- #check 0 #exit
--- 
--- end BitVec
--- 
--- namespace UInt8
--- 
--- @[simp]
--- def ofBit (b : Bit) : UInt8 :=
---   match b with
---   | 0 => 0
---   | 1 => 1
--- 
--- def lowestBit (x : UInt8) : Bit :=
---   .ofBool # Odd x.toNat
--- 
--- def ofBits (bs : List Bit) : UInt8 :=
---   bs.foldr (λ bit x => (x <<< 1) ||| ofBit bit) 0
--- 
--- def toBits (x : UInt8) : List Bit :=
---   List.range 8 |>.map # λ n => (x >>> ofNat n).lowestBit
--- 
--- -----
--- 
--- variable {x y z : UInt8}
--- variable {bs : List Bit}
--- 
--- attribute [simp] UInt8.toNat_lt_size
--- 
--- @[simp]
--- theorem mk_eq_mk_iff {x y : BitVec 8} : (⟨x⟩ : UInt8) = ⟨y⟩ ↔ x = y := by
---   constructor
---   · rintro ⟨⟩; rfl
---   · rintro rfl; rfl
--- 
--- @[simp]
--- theorem ofNatLT_eq_ofNatLT_iff {n m hn hm} : ofNatLT n hn = ofNatLT m hm ↔ n = m := by
---   simp_rw [ofNatLT, mk_eq_mk_iff]
---   simp
--- 
--- @[simp]
--- theorem ofBits_toBits : ofBits x.toBits = x := by
---   rcases x with ⟨v⟩
---   sorry
--- 
--- @[simp]
--- theorem toBits_eq_iff : x.toBits = y.toBits ↔ x = y := by
---   sorry
--- 
--- -- #check 0 #exit
--- 
--- @[simp]
--- theorem length_toBits : x.toBits.length = 8 := by
---   simp [toBits]
--- 
--- @[simp]
--- theorem list_subset_zero_one {bs : List Bit} : bs ⊆ [0, 1] := by
---   intro; simp
--- 
--- theorem toBits_ofBits_of_length_eq_8 (h : bs.length = 8) : (ofBits bs).toBits = bs := by
---   sorry
--- 
--- theorem toBits_ofBits_of_length_le_8 (h : bs.length ≤ 8) :
--- (ofBits bs).toBits = bs ++ List.replicate (8 - bs.length) 0 := by
---   sorry
--- 
--- @[simp]
--- theorem toBits_ne_nil : x.toBits ≠ [] := by
---   apply ne_of_congr (·.length); simp
--- 
--- @[simp]
--- theorem toBits_ofBits {bs : List Bit} :
--- (ofBits bs).toBits = bs ++ .replicate (8 - bs.length) 0 := by
---   simp [ofBits, toBits]
---   sorry
--- 
--- #check 0 #exit
--- 
--- end UInt8
--- 
--- namespace ByteArray
--- 
--- def ofBits' (acc : List UInt8) (bs : List Bit) : List UInt8 :=
---   if bs = [] then acc else
---   match _h : bs.splitAt 8 with
---   | (xs, bs') => ofBits' (.ofBits xs :: acc) bs'
--- termination_by bs.length
--- decreasing_by have : bs.length ≠ 0; simpa; grind
--- 
--- def ofBits (bs : List Bit) : ByteArray :=
---   ⟨⟨ofBits' [] bs |>.reverse⟩⟩
--- 
--- def toBits (bs : ByteArray) : List Bit :=
---   bs.1.1.flatMap UInt8.toBits
--- 
--- -----
--- 
--- theorem empty_def : (∅ : ByteArray) = ⟨⟨[]⟩⟩ := rfl
--- 
--- @[simp]
--- theorem ofBits_nil : ofBits [] = ∅ := by
---   ext <;> simp [ofBits, ofBits']
--- 
--- @[simp]
--- theorem ofBits'_nil {acc} : ofBits' acc [] = acc := by
---   simp [ofBits']
--- 
--- @[simp]
--- theorem ofBits_toBits {bs : ByteArray} : ofBits bs.toBits = bs := by
---   rcases bs with ⟨⟨bs⟩⟩
---   simp [ofBits, toBits]
---   suffices h : ∀ acc, ofBits' acc (bs.flatMap UInt8.toBits) = bs.reverse ++ acc
---   · specialize h []
---     simp at h
---     simp [h]
---   intro acc
---   induction bs generalizing acc
---   · simp
---   nm x bs ih
---   simp
---   unfold ofBits'
---   simp [ih]
--- 
--- theorem ofBits'_of_length_le_8 {bs₁ : List UInt8} {bs₂ : List Bit}
--- (h₁ : bs₂ ≠ []) (h₂ : bs₂.length ≤ 8) : ofBits' bs₁ bs₂ = .ofBits bs₂ :: bs₁ := by
---   unfold ofBits'; simp [h₁]; rw [List.take_eq_self_of_le h₂, List.drop_eq_nil_of_le h₂]; simp
--- 
--- @[simp] theorem toBits_empty : empty.toBits = [] := rfl
--- 
--- -- #check 0 #exit
--- 
--- @[simp]
--- theorem toBits_ofBits {bs : List Bit} :
--- (ofBits bs).toBits = bs ++ .replicate (bs.length % 8) 0 := by
---   generalize hn : bs.length = n
---   induction n using Nat.strong_induction_on generalizing bs
---   nm n ih; subst hn
---   by_cases h₁ : bs = []
---   ·
---     simp [h₁]
---   by_cases h₂ : bs.length < 8
---   ·
---     clear ih
---     rw [Nat.mod_eq_of_lt h₂]
---     simp [ofBits, toBits, ofBits'_of_length_le_8 h₁ # le_of_lt h₂]
--- 
--- #check 0 #exit
--- 
--- end ByteArray
--- 
--- structure Serializer where
---   bytes : ByteArray
---   curByte : UInt8
---   bitMask : UInt8
--- deriving DecidableEq
--- 
--- namespace Serializer
--- 
--- abbrev Ser := StateM Serializer
--- 
--- def empty : Serializer where
---   bytes := ∅
---   curByte := 0
---   bitMask := 1
--- 
--- instance : EmptyCollection Serializer := ⟨empty⟩
--- theorem empty_def : (∅ : Serializer) = empty := rfl
--- 
--- def flush' : Ser Unit := modify # λ s =>
---   { bytes := s.bytes.push s.curByte
---     curByte := 0
---     bitMask := 1
---   }
--- 
--- def flush : Ser Unit := do
---   bif (←get).bitMask != 0 then pure () else flush'
--- 
--- def writeBit' (b : Bit) : Ser Unit := modify # λ s =>
---   { bytes := s.bytes
---     curByte := match b with
---       | .B₀ => s.curByte
---       | .B₁ => s.curByte ||| s.bitMask
---     bitMask := s.bitMask <<< 1
---   }
--- 
--- def writeBit (b : Bit) : Ser Unit := do
---   writeBit' b; flush
--- 
--- def writeBits (bs : List Bit) : Ser Unit :=
---   bs.forM writeBit
--- 
--- def getOutput : Ser ByteArray := do
---   flush; gets (·.bytes)
--- 
--- def ofBits (bs : List Bit) : Serializer :=
---   StateT.run (m := Id) (writeBits bs) ∅ |>.2
--- 
--- -- #check 0 #exit
--- 
--- -----
--- 
--- variable {α β γ : Type}
--- variable {s : Serializer}
--- 
--- @[simp]
--- theorem writeBits_nil : writeBits [] = pure () := rfl
--- 
--- @[simp]
--- theorem getOutput_empty : getOutput.run ∅ = (∅, ∅) := rfl
--- 
--- @[simp low]
--- theorem writeBits_empty {bs} : (writeBits bs).run ∅ = ((), ofBits bs) := rfl
--- 
--- @[simp]
--- theorem ofBits_nil : ofBits [] = ∅ := rfl
--- 
--- @[simp]
--- theorem flush_empty : flush.run ∅ = ((), ∅) := rfl
--- 
--- @[simp]
--- theorem writeBits_cons {b bs} : writeBits (b :: bs) = (do writeBit b; writeBits bs) := rfl
--- 
--- @[simp]
--- theorem writeBits_append {bs₁ bs₂} :
--- writeBits (bs₁ ++ bs₂) = (do writeBits bs₁; writeBits bs₂) := by
---   simp [writeBits]
--- 
--- @[simp]
--- theorem flush_flush' : flush.run (flush'.run s).2 = flush'.run s := rfl
--- 
--- @[simp]
--- theorem flush_flush : flush.run (flush.run s).2 = flush.run s := by
---   nth_rw 2 [flush]; simp
---   split_ifs with h <;> simp
---   simp [flush, h]
--- 
--- @[simp]
--- theorem flush_ofBits {bs} : flush.run (ofBits bs) = ((), ofBits bs) := by
---   induction bs using List.reverseRecOn; simp
---   unfold ofBits; simp [writeBit, writeBit']; rfl
--- 
--- @[simp]
--- theorem getOutput_ofBits {bs} : getOutput.run (ofBits bs) = (ofBits bs |>.bytes, ofBits bs) := by
---   simp [getOutput]
--- 
--- @[simp]
--- theorem bytes_empty : (∅ : Serializer).bytes = ∅ := rfl
--- 
--- @[simp]
--- theorem ofBits_append {bs₁ bs₂} :
--- ofBits (bs₁ ++ bs₂) = (writeBits bs₂ |>.run (ofBits bs₁) |>.2) := by
---   unfold ofBits; simp
--- 
+
+-----
+
+variable {α β γ : Type}
+variable {s : Serializer}
+
+@[simp]
+theorem writeBits_nil : writeBits [] = pure () := rfl
+
+@[simp]
+theorem getOutput_empty : getOutput.run ∅ = (∅, ∅) := rfl
+
+@[simp low]
+theorem writeBits_empty {bs} : (writeBits bs).run ∅ = ((), ofBits bs) := rfl
+
+@[simp]
+theorem ofBits_nil : ofBits [] = ∅ := rfl
+
+@[simp]
+theorem flush_empty : flush.run ∅ = ((), ∅) := rfl
+
+@[simp]
+theorem writeBits_cons {b bs} : writeBits (b :: bs) = (do writeBit b; writeBits bs) := rfl
+
+@[simp]
+theorem writeBits_append {bs₁ bs₂} :
+writeBits (bs₁ ++ bs₂) = (do writeBits bs₁; writeBits bs₂) := by
+  simp [writeBits]
+
+@[simp]
+theorem flush_flush' : flush.run (flush'.run s).2 = flush'.run s := rfl
+
+@[simp]
+theorem flush_flush : flush.run (flush.run s).2 = flush.run s := by
+  nth_rw 2 [flush]; simp
+  split_ifs with h <;> simp
+  simp [flush, h]
+
+@[simp]
+theorem flush_ofBits {bs} : flush.run (ofBits bs) = ((), ofBits bs) := by
+  induction bs using List.reverseRecOn; simp
+  unfold ofBits; simp [writeBit, writeBit']; rfl
+
+@[simp]
+theorem getOutput_ofBits {bs} : getOutput.run (ofBits bs) = (ofBits bs |>.bytes, ofBits bs) := by
+  simp [getOutput]
+
+@[simp]
+theorem bytes_empty : (∅ : Serializer).bytes = ∅ := rfl
+
+@[simp]
+theorem ofBits_append {bs₁ bs₂} :
+ofBits (bs₁ ++ bs₂) = (writeBits bs₂ |>.run (ofBits bs₁) |>.2) := by
+  unfold ofBits; simp
+
 -- @[simp]
 -- theorem bytes_ofBits {bs : List Bit} : (ofBits bs).bytes = .ofBits bs := by
 --   generalize hn : bs.length = n
